[Yul] Fix bug in dynamic semantics.
Before this commit, the function environment was a finite map from function
names to function information (i.e. inputs, outputs, body), that was extended as
block were entered, also across function calls. However, when calling a
function, it is necessary to reduce the functions in the function environment to
the functions in scope for the called function.

Thus, the function environment is now a stack (i.e. list) of finite maps
(i.e. scopes), that is suitably reduced when calling functions. A function scope
is pushed when entering a block, and popped of zero or more scopes when calling
a function. Function environments are just recursively passed to the execution
functions; they are no longer threaded through, and so there is no need to pop
anything when exiting a block (we simply go back to the function environment
before the block.

At the same time, we have simplified the collection of the functions that form
the function scope to push onto the function environmetn stack, by first
filtering the function definitions out of the statement list in a block, and
then turning the list of function definitions into a function scope. The
resulting code is more orthogonal and clear.

books/kestrel/yul/language/dynamic-semantics.lisp
@@ -65,9 +65,7 @@
   (xdoc::topstring
    (xdoc::p
     "This is all the information about a function definition,
-     except for its name.
-     This is used for the values of function environments
-     (see @(tsee funenv)."))
+     except for its name."))
   ((inputs identifier-list)
    (outputs identifier-list)
    (body block))
@@ -90,31 +88,92 @@
 
 ;;;;;;;;;;;;;;;;;;;;;;;;;;;;;;;;;;;;;;;;;;;;;;;;;;;;;;;;;;;;;;;;;;;;;;;;;;;;;;;;
 
-(define funinfo-for-fundef ((fdef fundefp))
-  :returns (info funinfop)
+(define funinfo-for-fundef ((fundef fundefp))
+  :returns (funinfo funinfop)
   :short "Function information for a function definition."
-  (make-funinfo :inputs (fundef->inputs fdef)
-                :outputs (fundef->outputs fdef)
-                :body (fundef->body fdef))
+  :long
+  (xdoc::topstring
+   (xdoc::p
+    "This just takes the inputs, outputs, and body of the function definition
+     and forms function information with them."))
+  (make-funinfo :inputs (fundef->inputs fundef)
+                :outputs (fundef->outputs fundef)
+                :body (fundef->body fundef))
   :hooks (:fix))
 
 ;;;;;;;;;;;;;;;;;;;;;;;;;;;;;;;;;;;;;;;;;;;;;;;;;;;;;;;;;;;;;;;;;;;;;;;;;;;;;;;;
 
-(fty::defomap funenv
-  :short "Fixtype of function environments."
+(fty::defomap funscope
+  :short "Fixtype of function scopes."
   :long
   (xdoc::topstring
    (xdoc::p
     "This is a finite map from identifiers (function names)
      to function information:
-     it models the function definitions currently in scope;
-     this changes as blocks are entered and exited.
-     [Yul: Specification of Yul: Formal Specification]
-     does not explicitly mention this,
-     but its presence is implicit in the description of
-     the scope of function definitions."))
+     it models the function definitions in a scope."))
   :key-type identifier
   :val-type funinfo
+  :pred funscopep)
+
+;;;;;;;;;;;;;;;;;;;;;;;;;;;;;;;;;;;;;;;;
+
+(fty::defresult funscope-result
+  :short "Fixtype of errors and function scopes."
+  :ok funscope
+  :pred funscope-resultp)
+
+;;;;;;;;;;;;;;;;;;;;
+
+(defruled not-resulterrp-when-funscopep
+  (implies (funscopep x)
+           (not (resulterrp x)))
+  :enable resulterrp)
+
+;;;;;;;;;;;;;;;;;;;;;;;;;;;;;;;;;;;;;;;;;;;;;;;;;;;;;;;;;;;;;;;;;;;;;;;;;;;;;;;;
+
+(define funscope-for-fundefs ((fundefs fundef-listp))
+  :returns (funscope funscope-resultp)
+  :short "Function scope for a list of function definitions."
+  :long
+  (xdoc::topstring
+   (xdoc::p
+    "We go through the list and form a function scope for the functions.
+     It is an error if there are two functions with the same name."))
+  (b* (((when (endp fundefs)) nil)
+       ((ok scope) (funscope-for-fundefs (cdr fundefs)))
+       (fundef (car fundefs))
+       (fun (fundef->name fundef))
+       (fun+info (omap::in fun scope))
+       ((when (consp fun+info)) (err (list :duplicate-function fun))))
+    (omap::update fun (funinfo-for-fundef fundef) scope))
+  :hooks (:fix))
+
+;;;;;;;;;;;;;;;;;;;;;;;;;;;;;;;;;;;;;;;;;;;;;;;;;;;;;;;;;;;;;;;;;;;;;;;;;;;;;;;;
+
+(fty::deflist funenv
+  :short "Fixtype of function environments."
+  :long
+  (xdoc::topstring
+   (xdoc::p
+    "This is a list of function scopes,
+     which represents a stack;
+     the stack grows leftward, i.e.
+     push is @(tsee cons), pop is @(tsee cdr), and top is @(tsee car).
+     A function scope is pushed when entering a block,
+     and it is popped when exiting the block.
+     This needs to be a stack because Yul functions are statically scoped:
+     when a function later in the stack calls a function earlier in the stack,
+     the stack must be shrunk so that the called function
+     has access only to the functions that are statically in scope,
+     not the functions in inner blocks that the caller has access to.")
+   (xdoc::p
+    "[Yul: Specification of Yul: Formal Specification]
+     does not explicitly mention any notion of function environments,
+     but their presence is implicit in the description of
+     the scope of function definitions."))
+  :elt-type funscope
+  :true-listp t
+  :elementp-of-nil t
   :pred funenvp)
 
 ;;;;;;;;;;;;;;;;;;;;;;;;;;;;;;;;;;;;;;;;
@@ -133,69 +192,117 @@
 
 ;;;;;;;;;;;;;;;;;;;;;;;;;;;;;;;;;;;;;;;;;;;;;;;;;;;;;;;;;;;;;;;;;;;;;;;;;;;;;;;;
 
-(define get-fun ((fun identifierp) (funenv funenvp))
-  :returns (info funinfo-resultp)
-  :short "Obtain information about a function from the function environment."
+(fty::defprod funinfo+funenv
+  :short "Fixtype of pairs consisting of
+          function information and a function environment."
   :long
   (xdoc::topstring
    (xdoc::p
-    "It is an error if the function does not exist."))
-  (b* ((fun-info (omap::in (identifier-fix fun) (funenv-fix funenv)))
-       ((unless (consp fun-info))
-        (err (list :function-not-found (identifier-fix fun)))))
-    (cdr fun-info))
+    "These are used as (non-error) results of @(tsee get-fun):
+     see that function's documentation."))
+  ((info funinfo)
+   (env funenv)))
+
+;;;;;;;;;;;;;;;;;;;;;;;;;;;;;;;;;;;;;;;;
+
+(fty::defresult funinfo+funenv-result
+  :short "Fixtype of errors and
+          pairs consisting of
+          function information and a function environment."
+  :ok funinfo+funenv
+  :pred funinfo+funenv-resultp)
+
+;;;;;;;;;;;;;;;;;;;;
+
+(defruled not-resulterrp-when-funinfo+funenv-p
+  (implies (funinfo+funenv-p x)
+           (not (resulterrp x)))
+  :enable (resulterrp funinfo+funenv-p))
+
+;;;;;;;;;;;;;;;;;;;;;;;;;;;;;;;;;;;;;;;;;;;;;;;;;;;;;;;;;;;;;;;;;;;;;;;;;;;;;;;;
+
+(define find-fun ((fun identifierp) (funenv funenvp))
+  :returns (info funinfo+funenv-resultp)
+  :short "Find a function in the function environment by name."
+  :long
+  (xdoc::topstring
+   (xdoc::p
+    "We search through the scopes, from innermost to outermost.
+     It is an expected invariant that the scopes in a function environment
+     have disjoint function names
+     (we may formalize and prove this invariant at some point):
+     thus, the search order would not matter
+     if we only needed the function information;
+     however, as explained below, we also returned a function environment,
+     and therefore the innermost-to-outermost search order is important.")
+   (xdoc::p
+    "If we find @('fun'), we return not only its information,
+     but also the current function environment,
+     which is the initial function environment
+     with zero or more scopes popped;
+     the scope where @('fun') is found is not popped,
+     i.e. it is returned as the top scope.
+     This resulting function environment represents
+     the functions in scope for @('fun').
+     In @(tsee exec-function), which takes a @('fun') as argument,
+     we call @('find-fun') to retrieve the information about @('fun')
+     so that we can execute its body:
+     thus, it is convenient for @('find-fun') to return
+     the function environment for @('fun'),
+     which must be indeed passed to @(tsee exec-block) on the @('fun')'s body.")
+   (xdoc::p
+    "It is an error if @('fun') is not found in the environment."))
+  (b* (((when (endp funenv))
+        (err (list :function-not-found (identifier-fix fun))))
+       (funscope (funscope-fix (car funenv)))
+       (fun+info (omap::in (identifier-fix fun) funscope))
+       ((when (consp fun+info))
+        (make-funinfo+funenv :info (cdr fun+info) :env funenv)))
+    (find-fun fun (cdr funenv)))
   :hooks (:fix))
 
 ;;;;;;;;;;;;;;;;;;;;;;;;;;;;;;;;;;;;;;;;;;;;;;;;;;;;;;;;;;;;;;;;;;;;;;;;;;;;;;;;
 
-(define add-fun ((fun identifierp) (info funinfop) (funenv funenvp))
-  :returns (new-funenv funenv-resultp)
-  :short "Add a function to the function environment."
+(define ensure-funscope-disjoint ((funscope funscopep) (funenv funenvp))
+  :returns (_ resulterr-optionp)
+  :short "Ensure that a function scope is disjoint from a function environment."
   :long
   (xdoc::topstring
    (xdoc::p
-    "An error is returned if the function already exists.")
-   (xdoc::p
-    "This is the dynamic counterpart of
-     @(tsee add-funtype) in the static semantics."))
-  (b* ((fun-info (omap::in (identifier-fix fun) (funenv-fix funenv)))
-       ((when (consp fun-info))
-        (err (list :function-already-exists (identifier-fix fun))))
-       (new-funenv
-        (omap::update (identifier-fix fun)
-                      (funinfo-fix info)
-                      (funenv-fix funenv))))
-    new-funenv)
+    "That is, ensure that the function names in the scope
+     are disjoint from all the function names in the environment's scopes.
+     This is used to ensure that there is no function shadowing:
+     see @(tsee add-funs)."))
+  (b* (((when (endp funenv)) nil)
+       (overlap (set::intersect (omap::keys (funscope-fix funscope))
+                                (omap::keys (funscope-fix (car funenv)))))
+       ((unless (set::empty overlap))
+        (err (list :duplicate-functions overlap))))
+    (ensure-funscope-disjoint funscope (cdr funenv)))
   :hooks (:fix))
 
 ;;;;;;;;;;;;;;;;;;;;;;;;;;;;;;;;;;;;;;;;;;;;;;;;;;;;;;;;;;;;;;;;;;;;;;;;;;;;;;;;
 
-(define add-funs-in-statement-list ((stmts statement-listp) (funenv funenvp))
+(define add-funs ((fundefs fundef-listp) (funenv funenvp))
   :returns (new-funenv funenv-resultp)
-  :short "Add all the functions in a block to the function environment."
+  :short "Add functions to the function environment."
   :long
   (xdoc::topstring
    (xdoc::p
-    "Just before executing a block,
-     all the function definitions in the block
-     are added to the function environment.
-     This is because,
-     as explained in [Yul: Specification of Yul: Scoping Rules],
-     all the functions defined in a block are accessible in the whole block,
-     even before they are defined in the block.")
-   (xdoc::p
-    "This is the dynamic counterpart of
-     @(tsee add-funtypes-in-statement-list) in the static semantics."))
-  (b* (((when (endp stmts)) (funenv-fix funenv))
-       (stmt (car stmts))
-       ((unless (statement-case stmt :fundef))
-        (add-funs-in-statement-list (cdr stmts) funenv))
-       (fdef (statement-fundef->get stmt))
-       ((ok funenv) (add-fun (fundef->name fdef)
-                             (funinfo-for-fundef fdef)
-                             funenv)))
-    (add-funs-in-statement-list (cdr stmts) funenv))
-  :hooks (:fix))
+    "We create a function scope for the given list of function definitions
+     and we push that onto the function environment.
+     We ensure that the new functions have different names from
+     the functions already in the environment.
+     This ACL2 function is used for all the function definitions in a block;
+     see @(tsee exec-block)."))
+  (b* (((ok funscope) (funscope-for-fundefs fundefs))
+       ((ok &) (ensure-funscope-disjoint funscope funenv)))
+    (cons funscope (funenv-fix funenv)))
+  :hooks (:fix)
+  :prepwork
+  ((local
+    (in-theory
+     (enable funscopep-when-funscope-resultp-and-not-resulterrp)))))
 
 ;;;;;;;;;;;;;;;;;;;;;;;;;;;;;;;;;;;;;;;;;;;;;;;;;;;;;;;;;;;;;;;;;;;;;;;;;;;;;;;;
 
@@ -228,7 +335,7 @@
 ;;;;;;;;;;;;;;;;;;;;;;;;;;;;;;;;;;;;;;;;;;;;;;;;;;;;;;;;;;;;;;;;;;;;;;;;;;;;;;;;
 
 (fty::defprod cstate
-  :short "Fixtype of computational states."
+  :short "Fixtype of computation states."
   :long
   (xdoc::topstring
    (xdoc::p
@@ -668,11 +775,15 @@
        that takes values directly as arguments,
        in case we want to formally talk about function calls.")
      (xdoc::p
-      "We initialize the local state with the function's inputs and outputs.
-       We run the function body on the resulting computation state.
+      "We find the function in the function environment,
+       also obtaining the (generally smaller) function environment
+       for executing the function.
+       We initialize the local state with the function's inputs and outputs.
+       We run the function body on the resulting computation state
+       and on the function environment for executing the function.
        We read the final values of the function output variables
        and return them as result.
-       We also restore the computation state prior to the function call.")
+       We also restore the local state prior to the function call.")
      (xdoc::p
       "As a defensive check, we ensure that the function's body
        terminates regularly or via @('leave'),
@@ -680,11 +791,12 @@
     (b* (((when (zp limit)) (err (list :limit
                                    (identifier-fix fun)
                                    (value-list-fix args))))
+         ((ok (funinfo+funenv info+env)) (find-fun fun funenv))
+         ((funinfo info) info+env.info)
          (lstate-before (cstate->local cstate))
-         ((ok (funinfo info)) (get-fun fun funenv))
          ((ok cstate) (init-local info.inputs args info.outputs cstate))
          ((ok (soutcome outcome))
-          (exec-block info.body cstate funenv (1- limit)))
+          (exec-block info.body cstate info+env.env (1- limit)))
          ((when (mode-case outcome.mode :break))
           (err (list :break-from-function (identifier-fix fun))))
          ((when (mode-case outcome.mode :continue))
@@ -753,8 +865,7 @@
      (xdoc::p
       "For a loop statement,
        we start by saving (the names of) the variables before the loop,
-       similarly to @(tsee exec-block);
-       we also save the fucntion sate, similarly to @(tsee exec-block).
+       similarly to @(tsee exec-block).
        The initialization block of a loop statement
        is not treated like other blocks:
        its scope extends to the rest of the loop statement.
@@ -770,8 +881,6 @@
        We delegate the execution of the loop iterations
        to another ACL2 function.
        We take the result of that ACL2 function,
-       restore the function environment
-       (similarly to @(tsee exec-block),
        and remove the variables added by the loop
        (similarly to @(tsee exec-block)).")
      (xdoc::p
@@ -853,7 +962,7 @@
        :for
        (b* ((vars-before (omap::keys (cstate->local cstate)))
             (stmts (block->statements stmt.init))
-            ((ok funenv) (add-funs-in-statement-list stmts funenv))
+            ((ok funenv) (add-funs (statements-to-fundefs stmts) funenv))
             ((ok (soutcome outcome))
              (exec-statement-list stmts cstate funenv (1- limit)))
             ((when (mode-case outcome.mode :break))
@@ -932,17 +1041,14 @@
       "We save (the names of) the variables just before the block,
        so that we can restrict the computation state after the block
        to only those variables, as explained in @(tsee restrict-vars).
-       We also save the function environment before the block,
-       because we need to restore that after the block.
        We extend the function environment with the functions in the block.
        We execute the block's statements.
        We return the resulting outcome,
-       but we restore the function environment before the block
-       and we remove all the variables added by the block."))
+       but we remove all the variables added by the block."))
     (b* (((when (zp limit)) (err (list :limit (block-fix block))))
          (vars-before (omap::keys (cstate->local cstate)))
          (stmts (block->statements block))
-         ((ok funenv) (add-funs-in-statement-list stmts funenv))
+         ((ok funenv) (add-funs (statements-to-fundefs stmts) funenv))
          ((ok (soutcome outcome))
           (exec-statement-list stmts cstate funenv (1- limit)))
          (cstate (restrict-vars vars-before outcome.cstate)))
